minor updates for case study

MRiscX/AbstractSyntax/Registers.lean
@@ -9,21 +9,119 @@ def MRISCX_REG_SIZE : UInt64 := 32
 abbrev RegisterNr := Fin (MRISCX_REG_SIZE.toNat)
 
 namespace RegisterNr
-def ofNat (n:Nat) : RegisterNr := Fin.mk (n % MRISCX_REG_SIZE.toNat)
-                      (by
-                        apply Nat.mod_lt
-                        unfold MRISCX_REG_SIZE
-                        simp)
-def ofUInt64 (n:UInt64) : RegisterNr := Fin.mk (n.toNat % MRISCX_REG_SIZE.toNat)
-                          (by
-                            apply Nat.mod_lt
-                            unfold MRISCX_REG_SIZE
-                            simp)
+  def bareNames :=
+      [
+        "x0",
+        "x1",
+        "x2",
+        "x3",
+        "x4",
+        "x5",
+        "x6",
+        "x7",
+        "x8",
+        "x9",
+        "x10",
+        "x11",
+        "x12",
+        "x13",
+        "x14",
+        "x15",
+        "x16",
+        "x17",
+        "x18",
+        "x19",
+        "x20",
+        "x21",
+        "x22",
+        "x23",
+        "x24",
+        "x25",
+        "x26",
+        "x27",
+        "x28",
+        "x29",
+        "x30",
+        "x31"
+        ]
 
-def toUInt64 (r : RegisterNr) : UInt64 := UInt64.ofNat r.toNat
+    def abiNames :=
+      [
+        "zero",
+        "ra",
+        "sp",
+        "gp",
+        "tp",
+        "t0",
+        "t1",
+        "t2",
+        "s0",
+        "fp",
+        "s1",
+        "a0",
+        "a1",
+        "a2",
+        "a3",
+        "a4",
+        "a5",
+        "a6",
+        "a7",
+        "s2",
+        "s3",
+        "s4",
+        "s5",
+        "s6",
+        "s7",
+        "s8",
+        "s9",
+        "s10",
+        "s11",
+        "t3",
+        "t4",
+        "t5",
+        "t6"
+      ]
 
-instance InstRegisterNrOfNat (n : Nat) : OfNat RegisterNr n where
-  ofNat := RegisterNr.ofNat n
+  def isAbiName (str : String) :=
+    if RegisterNr.abiNames.contains str then
+      true
+    else
+      false
+
+
+  def isBareName (str : String) :=
+    if RegisterNr.bareNames.contains str then
+      true
+    else
+      false
+
+
+
+  def ofNat (n:Nat) : RegisterNr := Fin.mk (n % MRISCX_REG_SIZE.toNat)
+                        (by
+                          apply Nat.mod_lt
+                          unfold MRISCX_REG_SIZE
+                          simp)
+  def ofUInt64 (n:UInt64) : RegisterNr := Fin.mk (n.toNat % MRISCX_REG_SIZE.toNat)
+                            (by
+                              apply Nat.mod_lt
+                              unfold MRISCX_REG_SIZE
+                              simp)
+
+  def toUInt64 (r : RegisterNr) : UInt64 := UInt64.ofNat r.toNat
+
+  instance InstRegisterNrOfNat (n : Nat) : OfNat RegisterNr n where
+    ofNat := RegisterNr.ofNat n
+
+  def ofAbi? (str : String) : Option RegisterNr :=
+    if !isAbiName str then none
+    else
+      some (RegisterNr.ofNat (RegisterNr.abiNames.idxOf str))
+
+  def ofAbi! (str : String) (d : RegisterNr) : RegisterNr :=
+    match ofAbi? str with
+    | none => d
+    | some r => r
 
 end RegisterNr
 
@@ -43,97 +141,28 @@ instance : Inhabited RegisterName where
 
 namespace RegisterName
 
-  def bareNames :=
-    [
-      "x0",
-      "x1",
-      "x2",
-      "x3",
-      "x4",
-      "x5",
-      "x6",
-      "x7",
-      "x8",
-      "x9",
-      "x10",
-      "x11",
-      "x12",
-      "x13",
-      "x14",
-      "x15",
-      "x16",
-      "x17",
-      "x18",
-      "x19",
-      "x20",
-      "x21",
-      "x22",
-      "x23",
-      "x24",
-      "x25",
-      "x26",
-      "x27",
-      "x28",
-      "x29",
-      "x30",
-      "x31"
-      ]
-
-  def abiNames :=
-    [
-      "zero",
-      "ra",
-      "sp",
-      "gp",
-      "tp",
-      "t0",
-      "t1",
-      "t2",
-      "s0",
-      "fp",
-      "s1",
-      "a0",
-      "a1",
-      "a2",
-      "a3",
-      "a4",
-      "a5",
-      "a6",
-      "a7",
-      "s2",
-      "s3",
-      "s4",
-      "s5",
-      "s6",
-      "s7",
-      "s8",
-      "s9",
-      "s10",
-      "s11",
-      "t3",
-      "t4",
-      "t5",
-      "t6"
-    ]
 
   def beq (n₁ n₂ : RegisterName) := n₁.nr == n₂.nr
 
+  def ofAbi? (str : String) : Option RegisterName :=
+    match RegisterNr.ofAbi? str with
+    | none => none
+    | some r => RegisterName.mk r str
+
+  def ofAbi! (str : String) (d : RegisterName) :=
+    match ofAbi? str with
+    | none => d
+    | some n => n
+
+  def ofAbi!_zero (str : String) :=
+    match ofAbi? str with
+    | some n => n
+    | none => RegisterName.mk (RegisterNr.ofNat 0) ""
   -- def beq_regNr (n₁ n₂ : RegisterName) := n₁.nr  == n₂.nr
 
-  def isAbiName (str : String) :=
-    if abiNames.contains str then
-      true
-    else
-      false
-
-
-  def isBareName (str : String) :=
-    if bareNames.contains str then
-      true
-    else
-      false
 
 end RegisterName
+
 
 instance : BEq RegisterName where
   beq n1 n2 := RegisterName.beq n1 n2
